Generalize the ArrowP to Arrow conversion for any ffi Finish the implementation of the run mechanism for non-recursive functions

translator/monadic/cfMonadLib.sml
@@ -2,8 +2,58 @@ structure cfMonadLib (* :> cfMonadLib *) = struct
 
 open cfAppTheory cfTacticsLib ml_monad_translatorTheory cfMonadTheory
 
+val REF_REL_tm = ``REF_REL``;
+val RARRY_REL_tm = ``RARRAY_REL``;
+val emp_tm = ``emp : hprop``;
+fun prove_Hpred_Mem_Only H_def = let
+    val H = concl H_def |> lhs
+    val state_var = concl H_def |> rhs |> dest_abs |> fst
+    val state_type = type_of state_var
+    val hpreds = concl H_def |> rhs |> dest_abs |> snd |> list_dest dest_star
+
+    (* If H is `\state. emp` *)
+    val hpreds = if List.length hpreds = 1 andalso same_const emp_tm (List.hd hpreds) then []
+		 else hpreds
+
+    (* Prove the REFS_PRED_Mem_Only for every predicate *)
+    fun prove_mem_only h = let
+	val A = rator h |> rator |> rand
+	val r = rator h |> rand
+	val get_fun = mk_abs(state_var, rand h)
+	val pred = rator h |> rator |> rator
+			 
+	val th = if same_const REF_REL_tm pred then
+		     ISPECL [A, get_fun, r] REFS_PRED_Mem_Only_REF_REL
+		 else ISPECL [A, get_fun, r] REFS_PRED_Mem_Only_RARRAY_REL
+    in BETA_RULE th end
+    val interm_thms = List.map prove_mem_only hpreds
+
+    (* Assemble the predicates *)
+    fun apply_imp (th2, th1) = let
+	val H1 = concl th1 |> rand
+	val H2 = concl th2 |> rand
+
+	val th = ISPECL [H1, H2] REFS_PRED_Mem_Only_STAR_IMP
+	val th = MP (MP th th1) th2 |> BETA_RULE
+    in th end
+    val th = List.foldl apply_imp (List.hd interm_thms) (List.tl interm_thms)
+			|> PURE_REWRITE_RULE [GSYM H_def]
+             (* If H is `\state. emp` *)
+	     handle Empty => Thm.INST_TYPE [``:'a`` |-> state_type] REFS_PRED_Mem_Only_emp
+					   |> PURE_REWRITE_RULE [GSYM H_def]
+
+    (* Retrieve the final theorem *)
+    val imp_th = ISPEC H REFS_PRED_Mem_Only_IMP
+    val th = MP imp_th th
+
+    val p_var = concl th |> dest_forall |> fst
+    val tys = Type.match_type ``:'a ffi_proj`` (type_of p_var)
+    val tys = [Type.type_subst tys ``:'a`` |-> ``:unit``]
+    val unit_th = Thm.INST_TYPE tys th
+in (th, unit_th) end
+
 val PURE_tm = ``PURE : ('a -> v -> bool) -> ('a, 'b) H``;
-fun mk_app_of_ArrowP_goal spec = let
+fun mk_app_of_ArrowP_goal ffi spec = let
     val spec = PURE_REWRITE_RULE[ArrowM_def] spec
     val arrow_RI = concl spec |> rator |> rator
     val f_const = concl spec |> rator |> rand
@@ -12,7 +62,25 @@ fun mk_app_of_ArrowP_goal spec = let
     val state_type = type_of H |> dest_type |> snd |> List.hd
     val state_var = mk_var("state", state_type)
     val p_var = mk_var("p", ``:unit ffi_proj``)
+    val H_def = DB.find ((dest_const H |> fst) ^"_def") |> List.hd |> snd |> fst
 
+    (* Prove the assumptions on the STATE heap predicate *)
+    val (REFS_PRED_Mem_Only_thm, REFS_PRED_Mem_Only_unit_thm) = prove_Hpred_Mem_Only H_def
+    fun remove_mem_only_assums th = let
+	val target_p_var = concl th |> dest_imp |> fst |> dest_forall |> fst
+	val tys = Type.match_type ``:'a ffi_proj`` (type_of target_p_var)
+	val target_type = Type.type_subst tys ``:'a``
+
+	val origin_p_var = concl REFS_PRED_Mem_Only_thm |> dest_forall |> fst
+	val tys = Type.match_type ``:'a ffi_proj`` (type_of origin_p_var)
+	val origin_type = Type.type_subst tys ``:'a``
+
+	val inst_th = Thm.INST_TYPE [origin_type |-> target_type] REFS_PRED_Mem_Only_thm
+
+	val th = MP th inst_th
+	val th = MP th REFS_PRED_Mem_Only_unit_thm
+    in th end
+    
     (* Create variables for the HOL and CakeML parameters, retrieve the refinement invariants *)
     fun get_params arrow_RI n = let
 	val (comb_tm, params) = strip_comb arrow_RI
@@ -41,7 +109,7 @@ fun mk_app_of_ArrowP_goal spec = let
     val fv_var = mk_var("fv", ``:v``)
     val gv_var = mk_var("gv", ``:v``)
 
-    val th = ISPECL[last_ri, ret_inv, exn_inv, current_f, gv_var, H, last_x, last_xv, state_var] ArrowP_MONAD_to_app |> SPEC_ALL |> UNDISCH
+    val th = ISPECL[last_ri, ret_inv, exn_inv, current_f, gv_var, H, last_x, last_xv, state_var, ffi] ArrowP_MONAD_to_app |> remove_mem_only_assums |> UNDISCH
 
     val Q = concl th |> rand |> rand
     val Q_abs = mk_abs(state_var, Q)
@@ -56,8 +124,8 @@ fun mk_app_of_ArrowP_goal spec = let
 	val f_tm = concl th |> dest_imp |> fst |> rator |> rand |> rator
 	
 	val assum = GENL[state_var, gv_var] th
-	val imp_th = ISPECL[A, B, f_tm, fv_var, x, xv, xv2, xvl, H, Q_abs] ArrowP_PURE_to_app
-			|> SPEC_ALL |> UNDISCH |> BETA_RULE
+	val imp_th = ISPECL[A, B, f_tm, fv_var, x, xv, xv2, xvl, H, Q_abs, ffi] ArrowP_PURE_to_app
+			|> remove_mem_only_assums |> UNDISCH |> BETA_RULE
 	val th = MP imp_th assum |> SPEC_ALL |> Thm.INST [fv_var |-> gv_var]
     in mk_app_rec th x_info end
       | mk_app_rec th [] = th
