translator/monadic/cfMonadScript.sml
@@ -7,6 +7,8 @@ val _ = new_theory"cfMonad"
 
 val _ = Globals.max_print_depth := 40;
 
+val _ = hide "state";
+
 val HCOND_EXTRACT = cfLetAutoTheory.HCOND_EXTRACT;
 
 (*********** Comes from cfLetAutoLib.sml ***********************************************)	 
@@ -111,7 +113,7 @@ rw[]
 val st2heap_clock_inv = Q.prove(`st2heap p (st with clock := c) = st2heap p st`,
 Cases_on `p` \\ fs[st2heap_def]);
 
-val ArrowP_MONAD_to_app_basic_thm =  Q.store_thm("ArrowP_MONAD_to_app_basic_thm",
+val ArrowP_MONAD_to_app_basic_unit_thm =  Q.store_thm("ArrowP_MONAD_to_app_basic_unit_thm",
 `ArrowP H (PURE A) (MONAD B C) f fv ==>
 !refs x xv. A x xv ==>
 app_basic (p : unit ffi_proj) fv xv (H refs)
@@ -152,7 +154,7 @@ THENL[qexists_tac `Val a` \\ IMP_RES_TAC evaluate_Rval_bigStep_to_evaluate,
 \\ CONV_TAC ((STRIP_QUANT_CONV o RATOR_CONV) PURE_FACTS_FIRST_CONV)
 \\ fs[GSYM STAR_ASSOC, HCOND_EXTRACT]);
 
-val ArrowP_PURE_to_app_basic_thm =  Q.store_thm("ArrowP_PURE_to_app_basic_thm",
+(* val ArrowP_PURE_to_app_basic_unit_thm =  Q.store_thm("ArrowP_PURE_to_app_basic_unit_thm",
 `ArrowP H (PURE A) (PURE B) f fv ==>
 !refs x xv. A x xv ==>
 app_basic (p : unit ffi_proj) fv xv (H refs)
@@ -187,9 +189,9 @@ rw[]
 \\ fs[st2heap_clock_inv]
 \\ fs[SEP_EXISTS_THM]
 \\ fs[SEP_CLAUSES]
-\\ metis_tac[]);
+\\ metis_tac[]); *)
 
-val ArrowP_MONAD_to_app = Q.store_thm("ArrowP_MONAD_to_app",
+val ArrowP_MONAD_to_unit_app = Q.store_thm("ArrowP_MONAD_to_unit_app",
 `!A B C f fv H x xv refs p.
 A x xv ==>
 ArrowP H (PURE A) (MONAD B C) f fv ==>
@@ -198,9 +200,9 @@ app (p : unit ffi_proj) fv [xv] (H refs)
      (\rv. SEP_EXISTS refs' r. H refs' * &(f x refs = (Success r, refs')) * &(B r rv))
      (\ev. SEP_EXISTS refs' e. H refs' * &(f x refs = (Failure e, refs')) * &(C e ev)))`,
 rw[app_def]
-\\ metis_tac[ArrowP_MONAD_to_app_basic_thm]);
+\\ metis_tac[ArrowP_MONAD_to_app_basic_unit_thm]);
 
-val ArrowP_PURE_to_app = Q.store_thm("ArrowP_PURE_to_app",
+val ArrowP_PURE_to_unit_app = Q.store_thm("ArrowP_PURE_to_unit_app",
 `!A B f fv x1 xv1 xv2 xvl H Q p.
 A x1 xv1 ==>
 (!state gv. B (f x1) gv ==>
@@ -239,5 +241,363 @@ rw[app_def]
 \\ qexists_tac `{}`
 \\ fs[SPLIT_def, cond_def]
 \\ metis_tac[]);
+
+(*
+ * ffi of any type
+ *)
+
+val DISJ_TO_IMP = Q.prove(`(A \/ B) <=> ~A ==> B`,
+EQ_TAC >-(rw[] \\ rw[])
+\\ Cases_on `A`
+\\ rw[]);
+
+val INTER_DISJOINT = Q.store_thm("INTER_DISJOINT",
+`x IN h1 ==> x IN h2 ==> DISJOINT h1 h2 = F`,
+rw[]
+\\ rpt STRIP_TAC
+\\ fs[DISJOINT_DEF]
+\\ `(h1 INTER h2) x` by rw[INTER_DEF]
+\\ `{} x` by metis_tac[]
+\\ fs[]);
+
+val ArrowP_PURE_to_app = Q.store_thm("ArrowP_PURE_to_app",
+`!A B f fv x1 xv1 xv2 xvl H Q p.
+(!(p : 'a ffi_proj) st state h1 h2. SPLIT (st2heap p st) (h1, h2) ==> H state h1 ==> ?h3. SPLIT (store2heap st.refs) (h1, h3)) ==>
+(!(p : unit ffi_proj) st state h1 h2. SPLIT (st2heap p st) (h1, h2) ==> H state h1 ==> ?h3. SPLIT (store2heap st.refs) (h1, h3)) ==>
+A x1 xv1 ==>
+(!state gv. B (f x1) gv ==>
+app (p : 'a ffi_proj) gv (xv2::xvl) (H state) (Q state)) ==>
+(!state. ArrowP H (PURE A) (PURE B) f fv ==>
+app p fv (xv1::xv2::xvl) (H state) (Q state))`,
+rw[app_def]
+\\ rw[app_basic_def]
+\\ fs[ArrowP_def]
+\\ fs[PURE_def]
+\\ first_x_assum (qspec_then `x1` ASSUME_TAC)
+\\ POP_ASSUM IMP_RES_TAC
+\\ first_x_assum(qspecl_then[`empty_state with refs := st.refs`, `empty_state with refs := st.refs`, `[]`] ASSUME_TAC)
+\\ fs[state_component_equality]
+\\ sg `!p. ?h2. SPLIT (st2heap p (empty_state with refs := st.refs)) (h_i, h2)`
+>-(
+    last_x_assum IMP_RES_TAC
+    \\ rw[st2heap_def]
+    \\ qexists_tac `h3 UNION (ffi2heap p' empty_state.ffi)`
+    \\ fs[SPLIT_def, UNION_ASSOC]
+    \\ PURE_ONCE_REWRITE_TAC[DISJOINT_SYM]
+    \\ fs[]
+    \\ ASSUME_TAC (ISPECL [``p':unit ffi_proj``, ``empty_state with refs := st.refs``] st2heap_SPLIT_FFI)
+    \\ fs[SPLIT_def]
+    \\ qpat_x_assum `h_i UNION h3 = h` (fn x => fs[SYM x]))
+\\ first_x_assum(qspec_then `pu` STRIP_ASSUME_TAC)
+\\ IMP_RES_TAC REFS_PRED_lemma
+\\ qpat_x_assum `!refs1 p. R ==> ?env. R2` IMP_RES_TAC
+\\ POP_ASSUM(qspec_then `[]` STRIP_ASSUME_TAC)
+\\ fs[REFS_PRED_FRAME_def]
+\\ fs[evaluate_ck_def]
+\\ rw[]
+\\ `(H refs3 * (\s. s = h2)) (st2heap pu (empty_state with refs := st.refs))` by (rw[STAR_def] \\ SATISFY_TAC)
+\\ qpat_assum `!F. P` IMP_RES_TAC
+\\ IMP_RES_TAC HPROP_SPLIT3
+\\ fs[with_same_refs] \\ rw[]
+\\ IMP_RES_TAC evaluate_Rval_bigStep_to_evaluate
+\\ qexists_tac `Val v`
+\\ qexists_tac `h1`
+\\ qexists_tac `(st2heap p (st with refs := st.refs ++ junk)) DIFF h1 DIFF h_k`
+\\ qexists_tac `st with <| clock := 0; refs := st.refs ++ junk |>`
+\\ qexists_tac `c`
+\\ fs[SEP_CLAUSES, SEP_EXISTS_THM]
+\\ rw[]
+>-(
+    (* Clean up the assumptions *)
+    ntac 2 (POP_ASSUM (fn x => ALL_TAC))
+    \\ last_x_assum IMP_RES_TAC
+    \\ sg `SPLIT (st2heap pu (empty_state with refs := st.refs ++ junk)) (h1, h2 UNION h3)`
+    >-(fs[SPLIT_def, SPLIT3_def, UNION_ASSOC] \\ metis_tac[DISJOINT_SYM])
+    \\ last_x_assum IMP_RES_TAC
+    \\ fs[state_component_equality]
+    \\ ntac 2 (last_x_assum (fn x => ALL_TAC))
+    \\ last_x_assum ASSUME_TAC
+    \\ last_x_assum (fn x => ALL_TAC)
+    \\ last_x_assum ASSUME_TAC
+    \\ ntac 8 (last_x_assum (fn x => ALL_TAC))
+    \\ fs[SPLIT_def, SPLIT3_def]
+    \\ sg `!x. x IN h_i ==> x IN store2heap st.refs`
+    >-(
+	rw[]
+	\\ `x IN (h_i UNION h3''')` by fs[]
+	\\ metis_tac[UNION_DEF, IN_DEF])
+    \\ sg `h2 INTER (store2heap st.refs) = h_k INTER (store2heap st.refs)`
+    >-(
+	simp[SET_EQ_SUBSET, SUBSET_DEF]
+	\\ fs[st2heap_def]
+        \\ rw[]
+        >-(
+            `x IN h_i UNION h_k` by metis_tac[IN_UNION]
+            \\ fs[]
+            \\ IMP_RES_TAC INTER_DISJOINT)
+        \\ `x IN h_i UNION h2` by metis_tac[IN_UNION]
+        \\ fs[]
+        \\ IMP_RES_TAC INTER_DISJOINT)
+    \\ reverse(rw[])
+    >-(
+	rw[DISJOINT_DEF]
+	\\ PURE_ONCE_REWRITE_TAC[GSYM SUBSET_EMPTY]
+	\\ PURE_REWRITE_TAC[SUBSET_DEF]
+	\\ rpt STRIP_TAC
+	\\ fs[]
+	\\ metis_tac[])
+    >-(
+	rw[DISJOINT_DEF]
+	\\ PURE_ONCE_REWRITE_TAC[GSYM SUBSET_EMPTY]
+	\\ PURE_REWRITE_TAC[SUBSET_DEF]
+	\\ rpt STRIP_TAC
+	\\ fs[]
+	\\ metis_tac[])
+    (* DISJOINT h1 h_k *)
+    >-(
+	rw[DISJOINT_ALT]
+	\\ rw[]
+	\\ `x IN store2heap (st.refs ++ junk)` by metis_tac[IN_UNION]
+	\\ fs[cfAppTheory.store2heap_append_many]
+	>-(
+	    strip_tac
+            \\ `x IN h2` by metis_tac[IN_INTER]
+            \\ fs[DISJOINT_ALT]
+	    \\ metis_tac[])
+	>-(
+	    strip_tac
+	    \\ `x IN (st2heap p st)` by metis_tac[IN_UNION]
+	    \\ fs[st2heap_def]
+	    >-(
+		`SPLIT (store2heap (st.refs ++ junk)) (store2heap st.refs, store2heap_aux (LENGTH st.refs) junk)` by fs[store2heap_SPLIT]
+		\\ fs[SPLIT_def]
+		\\ fs[DISJOINT_ALT])
+	    \\ Cases_on `x`
+	    \\ fs[Mem_NOT_IN_ffi2heap, FFI_split_NOT_IN_store2heap_aux, FFI_full_NOT_IN_store2heap_aux, FFI_part_NOT_IN_store2heap_aux]))
+    (* SETS EQUALITY *)
+    \\ simp[Once SET_EQ_SUBSET, SUBSET_DEF]
+    \\ fs[st2heap_clock]
+    \\ rw[]
+    >-(
+	sg `x IN store2heap (st.refs ++ junk)`
+	>-(
+	    fs[st2heap_def, cfAppTheory.store2heap_append_many]
+	    \\ `x IN h1 ∪ h3''` by fs[]
+	    \\ `x IN store2heap st.refs ∪ store2heap_aux (LENGTH st.refs) junk` by metis_tac[]
+	    \\ fs[])
+	\\ rw[st2heap_def])
+    >-(
+	sg `x IN st2heap p st`
+	>-(
+	    `x IN h_i ∪ h_k` by fs[]
+	    \\ metis_tac[])
+	\\ rw[st2heap_def]
+	\\ fs[st2heap_def, cfAppTheory.store2heap_append_many])
+    \\ Cases_on `x IN h1` >> fs[]
+    \\ Cases_on `x IN h_k` >> fs[]
+    \\ fs[IN_DEF, st2heap_def])
+>-(qexists_tac `H refs3` \\ fs[HCOND_EXTRACT])
+\\ ASSUME_TAC (Thm.INST_TYPE[``:'a`` |-> ``:unit``, ``:'b`` |-> ``:'a``] (CONJUNCT1 evaluatePropsTheory.evaluate_ffi_intro))
+\\ first_x_assum IMP_RES_TAC
+\\ fs[state_component_equality, ml_translatorTheory.empty_state_def, ffiTheory.initial_ffi_state_def]);
+
+val prove_ArrowP_MONAD_to_app_SPLIT3 = ntac 2 (POP_ASSUM (fn x => ALL_TAC))
+  \\ last_x_assum IMP_RES_TAC
+  \\ sg `SPLIT (st2heap pu (empty_state with refs := refs')) (h1, h2 UNION h3)`
+  >-(fs[SPLIT_def, SPLIT3_def, UNION_ASSOC] \\ metis_tac[DISJOINT_SYM])
+  \\ last_x_assum IMP_RES_TAC
+  \\ last_x_assum (fn x => ALL_TAC)
+  \\ fs[state_component_equality, st2heap_clock]
+  \\ ntac 3 (last_x_assum ASSUME_TAC)
+  \\ ntac 6 (last_x_assum (fn x => ALL_TAC))
+  \\ fs[SPLIT_def, SPLIT3_def]
+  \\ `!x. x IN h_i ==> x IN store2heap st.refs` by metis_tac[IN_UNION]
+  \\ sg `h2 INTER (store2heap refs') = h_k INTER (store2heap refs')`
+  >-(
+      simp[SET_EQ_SUBSET, SUBSET_DEF]
+      \\ fs[st2heap_def]
+      \\ rw[]
+      >-(
+	  sg `x IN store2heap st.refs`
+	  >-(
+	      `x IN store2heap st.refs UNION ffi2heap pu empty_state.ffi` by metis_tac[IN_UNION]
+	      \\ Cases_on `x`
+	      >> fs[store2heap_def, Mem_NOT_IN_ffi2heap, FFI_split_NOT_IN_store2heap_aux, FFI_full_NOT_IN_store2heap_aux, FFI_part_NOT_IN_store2heap_aux])
+	  \\ `x IN h_i ∪ h_k` by metis_tac[IN_UNION]
+	  \\ fs[]
+	  \\ IMP_RES_TAC INTER_DISJOINT)
+      \\ sg `x IN store2heap st.refs`
+	  >-(
+	     `x IN store2heap st.refs UNION ffi2heap p st.ffi` by metis_tac[IN_UNION]
+	     \\ Cases_on `x`
+	     >> fs[store2heap_def, Mem_NOT_IN_ffi2heap, FFI_split_NOT_IN_store2heap_aux, FFI_full_NOT_IN_store2heap_aux, FFI_part_NOT_IN_store2heap_aux])
+      \\ `x IN h_i ∪ h2` by metis_tac[IN_UNION]
+      \\ fs[]
+      \\ IMP_RES_TAC INTER_DISJOINT)
+  \\ sg `h2 INTER (store2heap st.refs) = h_k INTER (store2heap st.refs)`
+  >-(
+      simp[SET_EQ_SUBSET, SUBSET_DEF]
+      \\ fs[st2heap_def]
+      \\ rw[]
+      >-(
+	  `x IN h_i UNION h_k` by metis_tac[IN_UNION]
+	  \\ fs[]
+	  \\ IMP_RES_TAC INTER_DISJOINT)
+      \\ `x IN h_i UNION h2` by metis_tac[IN_UNION]
+      \\ fs[]
+      \\ IMP_RES_TAC INTER_DISJOINT)
+  \\ reverse(rw[])
+  >-(
+      rw[DISJOINT_DEF]
+      \\ PURE_ONCE_REWRITE_TAC[GSYM SUBSET_EMPTY]
+      \\ PURE_REWRITE_TAC[SUBSET_DEF]
+      \\ rpt STRIP_TAC
+      \\ fs[]
+      \\ metis_tac[])
+  >-(
+      rw[DISJOINT_DEF]
+      \\ PURE_ONCE_REWRITE_TAC[GSYM SUBSET_EMPTY]
+      \\ PURE_REWRITE_TAC[SUBSET_DEF]
+      \\ rpt STRIP_TAC
+      \\ fs[]
+      \\ metis_tac[])
+  (* DISJOINT h1 h_k *)
+  >-(
+      rw[DISJOINT_ALT]
+      \\ rw[]
+      \\ `x IN store2heap refs'` by metis_tac[IN_UNION]
+      \\ strip_tac
+      \\ `x IN h2` by metis_tac[IN_UNION, IN_INTER]
+      \\ IMP_RES_TAC INTER_DISJOINT)
+  (* SETS EQUALITY *)
+  \\ simp[Once SET_EQ_SUBSET, SUBSET_DEF]
+  \\ reverse(rw[])
+  >-(metis_tac[])
+  >-(
+      `x IN st2heap p st` by metis_tac[IN_UNION]
+      \\ fs[st2heap_def]
+      \\ `x IN store2heap refs' ∪ ffi2heap pu empty_state.ffi` by metis_tac[IN_UNION, UNION_ASSOC, IN_INTER]
+      \\ fs[]
+      \\ irule FALSITY
+      \\ Cases_on `x`
+      >> fs[store2heap_def, Mem_NOT_IN_ffi2heap, FFI_split_NOT_IN_store2heap_aux, FFI_full_NOT_IN_store2heap_aux, FFI_part_NOT_IN_store2heap_aux])
+  \\ fs[st2heap_def]
+  \\ metis_tac[IN_UNION];
+
+val ArrowP_MONAD_to_app = Q.store_thm("ArrowP_MONAD_to_app",
+`!A B C f fv H x xv refs p.
+(!(p : 'a ffi_proj) st state h1 h2. SPLIT (st2heap p st) (h1, h2) ==> H state h1 ==> ?h3. SPLIT (store2heap st.refs) (h1, h3)) ==>
+(!(p : unit ffi_proj) st state h1 h2. SPLIT (st2heap p st) (h1, h2) ==> H state h1 ==> ?h3. SPLIT (store2heap st.refs) (h1, h3)) ==>
+A x xv ==>
+ArrowP H (PURE A) (MONAD B C) f fv ==>
+app (p : 'a ffi_proj) fv [xv] (H refs)
+(POST
+     (\rv. SEP_EXISTS refs' r. H refs' * &(f x refs = (Success r, refs')) * &(B r rv))
+     (\ev. SEP_EXISTS refs' e. H refs' * &(f x refs = (Failure e, refs')) * &(C e ev)))`,
+rw[app_def]
+\\ rw[app_basic_def]
+\\ fs[ArrowP_def]
+\\ fs[PURE_def]
+\\ first_x_assum (qspec_then `x` ASSUME_TAC)
+\\ POP_ASSUM IMP_RES_TAC
+\\ fs[state_component_equality]
+\\ first_x_assum(qspecl_then[`empty_state with refs := st.refs`, `[]`] ASSUME_TAC)
+\\ sg `!p. ?h2. SPLIT (st2heap p (empty_state with refs := st.refs)) (h_i, h2)`
+>-(
+    last_x_assum IMP_RES_TAC
+    \\ last_x_assum IMP_RES_TAC
+    \\ rw[st2heap_def]
+    \\ qexists_tac `h3 UNION (ffi2heap p' empty_state.ffi)`
+    \\ fs[SPLIT_def, UNION_ASSOC]
+    \\ PURE_ONCE_REWRITE_TAC[DISJOINT_SYM]
+    \\ fs[]
+    \\ rw[DISJOINT_ALT]
+    \\ sg `x' IN store2heap st.refs`
+    >-(
+	`x' IN h_i UNION h3` by fs[]
+        \\ metis_tac[])
+    \\ fs[store2heap_def]
+    \\ Cases_on `x'`
+    >> fs[Mem_NOT_IN_ffi2heap, FFI_split_NOT_IN_store2heap_aux, FFI_full_NOT_IN_store2heap_aux, FFI_part_NOT_IN_store2heap_aux])
+\\ first_x_assum(qspec_then `pu` STRIP_ASSUME_TAC)
+\\ IMP_RES_TAC REFS_PRED_lemma
+\\ qpat_x_assum `!refs1 p. R ==> ?env. R2` IMP_RES_TAC
+\\ POP_ASSUM(qspec_then `[]` STRIP_ASSUME_TAC)
+\\ fs[REFS_PRED_FRAME_def]
+\\ fs[evaluate_ck_def]
+\\ rw[]
+\\ `(H refs * (\s. s = h2)) (st2heap pu (empty_state with refs := st.refs))` by (rw[STAR_def] \\ SATISFY_TAC)
+\\ qpat_assum `!F. P` IMP_RES_TAC
+\\ IMP_RES_TAC HPROP_SPLIT3
+\\ fs[with_same_refs] \\ rw[]
+\\ Cases_on `res3`
+>> Cases_on `f x refs`
+>> Cases_on `q`
+>> fs[MONAD_def]
+THENL[ALL_TAC, Cases_on `e`]
+>> fs[]
+THENL[IMP_RES_TAC evaluate_Rval_bigStep_to_evaluate \\ qexists_tac `Val a`,
+      IMP_RES_TAC evaluate_Rerr_bigStep_to_evaluate \\ qexists_tac `Exn a`]
+\\ qexists_tac `h1`
+\\ qexists_tac `(st2heap p (st with refs := refs')) DIFF h1 DIFF h_k`
+\\ qexists_tac `st with <| clock := 0; refs := refs' |>`
+\\ qexists_tac `c`
+\\ fs[SEP_CLAUSES, SEP_EXISTS_THM]
+\\ rw[]
+>-(prove_ArrowP_MONAD_to_app_SPLIT3)
+>-(fs[HCOND_EXTRACT])
+>-(
+    ASSUME_TAC (Thm.INST_TYPE[``:'a`` |-> ``:unit``, ``:'b`` |-> ``:'a``] (CONJUNCT1 evaluatePropsTheory.evaluate_ffi_intro))
+    \\ first_x_assum IMP_RES_TAC
+    \\ fs[state_component_equality, ml_translatorTheory.empty_state_def, ffiTheory.initial_ffi_state_def])
+>-(prove_ArrowP_MONAD_to_app_SPLIT3)
+>-(fs[HCOND_EXTRACT])
+\\ ASSUME_TAC (Thm.INST_TYPE[``:'a`` |-> ``:unit``, ``:'b`` |-> ``:'a``] (CONJUNCT1 evaluatePropsTheory.evaluate_ffi_intro))
+\\ first_x_assum IMP_RES_TAC
+\\ fs[state_component_equality, ml_translatorTheory.empty_state_def, ffiTheory.initial_ffi_state_def]);
+
+val REFS_PRED_Mem_Only_def = Define `REFS_PRED_Mem_Only H = !state h. H state h ==> !x. x IN h ==> ?n v. x = Mem n v`;
+
+val REFS_PRED_Mem_Only_IMP = Q.store_thm("REFS_PRED_Mem_Only_IMP",
+`!H. REFS_PRED_Mem_Only H ==> ((!p st state h1 h2. SPLIT (st2heap p st) (h1, h2) ==> H state h1 ==> ?h3. SPLIT (store2heap st.refs) (h1, h3)))`,
+rw[REFS_PRED_Mem_Only_def]
+\\ fs[SPLIT_def]
+\\ qexists_tac `store2heap st.refs DIFF h1`
+\\ rw[]
+>-(
+    rw[SET_EQ_SUBSET, SUBSET_DEF]
+    \\ `x IN st2heap p st` by metis_tac[IN_UNION]
+    \\ fs[st2heap_def]
+    \\ last_x_assum IMP_RES_TAC
+    \\ fs[Mem_NOT_IN_ffi2heap])
+\\ fs[DISJOINT_ALT]);
+
+val REFS_PRED_Mem_Only_STAR_IMP = Q.store_thm("REFS_PRED_Mem_Only_STAR_IMP",
+`!H1 H2. REFS_PRED_Mem_Only H1 ==> REFS_PRED_Mem_Only H2 ==> REFS_PRED_Mem_Only (\state. H1 state * H2 state)`,
+rw[REFS_PRED_Mem_Only_def]
+\\ fs[STAR_def, SPLIT_def]
+\\ metis_tac[IN_DEF, IN_UNION]);
+
+val REFS_PRED_Mem_Only_REF_REL = Q.store_thm("REFS_PRED_Mem_Only_REF_REL",
+`!A get_val r. REFS_PRED_Mem_Only (\state. REF_REL A r (get_val state))`,
+rw[REFS_PRED_Mem_Only_def]
+\\ fs[REF_REL_def, SEP_EXISTS_THM, HCOND_EXTRACT, REF_def, cell_def, one_def]
+\\ rw[]
+\\ fs[IN_SING]);
+
+val REFS_PRED_Mem_Only_RARRAY_REL = Q.store_thm("REFS_PRED_Mem_Only_RARRAY_REL",
+`!A get_arr r. REFS_PRED_Mem_Only (\state. RARRAY_REL A r (get_arr state))`,
+rw[REFS_PRED_Mem_Only_def]
+\\ fs[RARRAY_REL_def, RARRAY_def, ARRAY_def, SEP_CLAUSES, SEP_EXISTS_THM, HCOND_EXTRACT, REF_def, cell_def, one_def, GSYM STAR_ASSOC]
+\\ fs[STAR_def, SPLIT_def, cond_def]
+\\ rw[]
+\\ fs[IN_SING]);
+
+val REFS_PRED_Mem_Only_emp = Q.store_thm("REFS_PRED_Mem_Only_emp",
+`REFS_PRED_Mem_Only (\(state : 'a). emp)`,
+rw[REFS_PRED_Mem_Only_def]
+\\ fs[REF_REL_def, SEP_EXISTS_THM, HCOND_EXTRACT, REF_def, cell_def, one_def, emp_def]
+\\ rw[]
+\\ fs[]);
 
 val _ = export_theory();
