translator/monadic/examples/runProgScript.sml
@@ -55,12 +55,17 @@ val array_manip_funs = define_Marray_manip_funs array_access_funs sub_exn update
 
 (* Prepare the translation *)
 val init_num_def = Define `init_num = (0 : num)`;
-val refs_init_list = [(the_num_name, init_num_def, get_the_num_def, set_the_num_def)];
-
 val init_num_array_def = Define `init_num_array = [] : num list`;
 val init_int_array_def = Define `init_int_array = [] : int list`;
+val refs_init_list = [(the_num_name, init_num_def, get_the_num_def, set_the_num_def),
+		     (the_num_array_name, init_num_array_def, get_the_num_array_def, set_the_num_array_def),
+		     (the_int_array_name, init_int_array_def, get_the_int_array_def, set_the_int_array_def)];
+(* val refs_init_list = [(the_num_name, init_num_def, get_the_num_def, set_the_num_def)]; *)
+
+(* val init_num_array_def = Define `init_num_array = [] : num list`;
+val init_int_array_def = Define `init_int_array = [] : int list`;
 val arrays_init_values = [init_num_array_def, init_int_array_def];
-val arrays_init_list = List.map (fn ((x1, x2, x3, x4, x5, x6, x7), x) => (x1, x, x2, x3, x4, x5, x6, x7)) (zip array_manip_funs arrays_init_values);
+val arrays_init_list = List.map (fn ((x1, x2, x3, x4, x5, x6, x7), x) => (x1, x, x2, x3, x4, x5, x6, x7)) (zip array_manip_funs arrays_init_values); *)
 
 val infer_init_state = ``<|the_num := 0; the_num_array := []; the_int_array := []|>``;
 
@@ -70,7 +75,8 @@ val EXN_RI = ``STATE_EXN_TYPE``;
 val exn_ri_def = STATE_EXN_TYPE_def;
 
 val refs_manip_list = List.map (fn (x, _, y, z) => (x, y, z)) refs_init_list;
-val arrays_manip_list = List.map (fn (x1, _, x2, x3, x4, x5, x6, x7) => (x1, x2, x3, x4, x5, x6, x7)) arrays_init_list;
+(* val arrays_manip_list = List.map (fn (x1, _, x2, x3, x4, x5, x6, x7) => (x1, x2, x3, x4, x5, x6, x7)) arrays_init_list; *)
+val arrays_manip_list = [] : (string * thm * thm * thm * thm * thm * thm) list;
 
 val translation_parameters = translate_dynamic_init_fixed_store refs_manip_list arrays_manip_list store_hprop_name state_type exn_ri_def;
 
@@ -80,14 +86,14 @@ val translation_parameters = translate_dynamic_init_fixed_store refs_manip_list 
 (* Initialize the translation *)
 (* val store_pred_exists = SOME(#store_pred_exists_thm store_trans_result); *)
 val store_pred_exists = NONE : thm option;
-val _ = init_translation translation_parameters store_pred_exists exc_ri_def [];
+val _ = init_translation translation_parameters store_pred_exists exn_ri_def [];
 
 (* Prove the theorems necessary to handle the exceptions *)
 val (raise_functions, handle_functions) = unzip exceptions_funs;
 val exn_thms = add_raise_handle_functions raise_functions handle_functions STATE_EXN_TYPE_def
 
 (* Monadic translations *)
-val test2_def = Define `test2 n = the_num_array_sub n`;
+(* val test2_def = Define `test2 n = the_num_array_sub n`;
 val def = test2_def |> m_translate;
 
 val test3_def = Define `test3 n x = update_the_num_array n x`;
@@ -117,16 +123,22 @@ val test7_v_th = m_translate test7_def;
 
 val test8_def = Define `
 test8 l = test7 l`;
-val test8_v_th = m_translate test8_def;
+val test8_v_th = m_translate test8_def; *)
 
-val test9_def = Define `
-test9 n m z =
+val test1_def = Define `test1 x = do y <- get_the_num; return (x + y) od`;
+val test1_v_th = m_translate test1_def;
+
+val test2_def = Define `test2 (x : num) y = return (x + y)`;
+val test2_v_th = m_translate test2_def;
+
+val test3_def = Define `
+test3 n m z =
    do
-       test5 n z;
-       x <- test2 m;
+       test2 n z;
+       x <- test1 m;
        return x
    od`;
-val test9_v_th = m_translate test9_def;
+val test3_v_th = m_translate test3_def;
 
 (* New definitions for ml_monadBaseTheory *)
 val _ = ParseExtras.temp_tight_equality();
@@ -137,189 +149,15 @@ fun evaluate_unique_result_tac (g as (asl, w)) = let
 in simp uniques g end;
 
 (* Test *)
-set_trace "assumptions" 1
-
 val current_state = get_state(get_ml_prog_state());
 val current_env = get_env(get_ml_prog_state());
 
-val spec = test9_v_th
+val spec = test3_v_th
 val original_spec = spec;
 
-val spec_info_pat = ``nsLookup (merge_env (LOCAL_ENV : v sem_env) env).v (Short NAME) = SOME EXPR``;
+val run_test_def = Define `run_test n m z refs = run (test3 n m z) refs`;
+val def = run_test_def;
 
-
-val initial_state = mk_var("s", ``:unit semanticPrimitives$state``);
-
-val (name, def) = List.hd ref_name_def_pairs;
-
-val evaluate_let_opref = Q.store_thm("evaluate_let_opref",
-`Eval env exp1 P ==>
-?junk v. evaluate F env s (Let (SOME vname) (App Opref [exp1]) exp2) = evaluate F (write vname (Loc (LENGTH (s.refs ++ junk))) env) (s with refs := s.refs ++ junk ++ [Refv v]) exp2 /\ P v`,
-rw[Eval_def]
-\\ first_x_assum(qspec_then `s.refs` STRIP_ASSUME_TAC)
-\\ IMP_RES_TAC evaluate_empty_state_IMP
-\\ qexists_tac `refs'`
-\\ qexists_tac `res`
-\\ simp[]
-\\ irule EQ_EXT
-\\ rw[Once evaluate_cases]
-\\ rw[Once evaluate_cases]
-\\ rw[Once evaluate_cases]
-\\ evaluate_unique_result_tac
-\\ rw[Once evaluate_cases]
-\\ rw[do_app_def, store_alloc_def]
-\\ fs[write_def, namespaceTheory.nsOptBind_def]
-\\ rw[Once DISJ_COMM]
-\\ rw[Once evaluate_cases]
-\\ rw[Once evaluate_cases]
-\\ evaluate_unique_result_tac
-\\ rw[Once evaluate_cases]
-\\ rw[do_app_def, store_alloc_def]
-\\ rw[Once evaluate_cases]
-\\ evaluate_unique_result_tac
-\\ rw[Once evaluate_cases]
-\\ rw[Once evaluate_cases]
-\\ evaluate_unique_result_tac
-\\ rw[Once evaluate_cases]
-\\ rw[with_same_ffi]);
-
-val EvalSt_Let_Fun = Q.store_thm("EvalSt_Let_Fun",
-`EvalSt (merge_env (write vname (Closure (merge_env env1 env0) xv fexp) env1) env0) exp P refs H ==>
-EvalSt (merge_env env1 env0) (Let (SOME vname) (Fun xv fexp) exp) P refs H`,
-rw[EvalSt_def]
-\\ last_x_assum IMP_RES_TAC
-\\ first_x_assum(qspec_then `junk` STRIP_ASSUME_TAC)
-\\ rw[Once evaluate_cases]
-\\ rw[Once evaluate_cases]
-\\ rw[namespaceTheory.nsOptBind_def]
-\\ fs[write_def, merge_env_def]
-\\ metis_tac[]);
-
-val merge_env_bind_empty = Q.store_thm("merge_env_bind_empty",
-`merge_env <| v := Bind [] []; c := Bind [] [] |> env  = env`,
-rw[merge_env_def]
-\\ Cases_on `env`
-\\ Cases_on `n`
-\\ Cases_on `n0`
-\\ rw[namespaceTheory.nsAppend_def, sem_env_component_equality]);
-
-val EvalSt_Opref = Q.store_thm("EvalSt_Opref",
-`Eval (merge_env <|v := Bind binds []; c := Bind [] []|> env0) state_exp (STATE_TYPE state) ==>
-Eval (merge_env <| v := Bind binds []; c := Bind [] [] |> env0) get_ref_expr ((STATE_TYPE --> TYPE) (\state. get_val state)) ==>
-(!loc. EvalSt (merge_env <| v := Bind ((loc_name, loc)::binds) []; c := Bind [] [] |> env0) exp P state (\state. REF_REL TYPE loc (get_val state) * H state)) ==>
-EvalSt (merge_env <| v := Bind binds []; c := Bind [] [] |> env0)
-(Let (SOME loc_name) (App Opref [App Opapp [get_ref_expr; state_exp]]) exp) P state (\state. H state)`,
-rw[EvalSt_def]
-\\ rw[Once evaluate_cases]
-\\ rw[Once evaluate_cases]
-\\ rw[Once evaluate_cases]
-\\ fs[Eval_def]
-\\ last_x_assum(qspec_then `s.refs ++ junk` STRIP_ASSUME_TAC)
-\\ first_x_assum(fn x => MATCH_MP evaluate_empty_state_IMP_junk x |> ASSUME_TAC)
-\\ evaluate_unique_result_tac
-\\ rw[Once evaluate_cases]
-\\ last_x_assum(qspec_then `s.refs ++ junk ++ refs'` STRIP_ASSUME_TAC)
-\\ FULL_SIMP_TAC pure_ss [GSYM APPEND_ASSOC]
-\\ `s.refs ++ (junk ++ (refs' ++ refs'')) = s.refs ++ (junk ++ refs') ++ refs''` by simp[]
-\\ pop_assum(fn x => FULL_SIMP_TAC pure_ss [x])
-\\ first_x_assum(fn x => MATCH_MP evaluate_empty_state_IMP_junk x |> ASSUME_TAC)
-\\ rw[Once evaluate_cases]
-\\ evaluate_unique_result_tac
-\\ rw[Once evaluate_cases]
-\\ fs[Arrow_def]
-\\ first_x_assum(qspec_then `state` ASSUME_TAC)
-\\ fs[AppReturns_def]
-\\ first_x_assum(qspec_then `res` IMP_RES_TAC)
-\\ first_x_assum(qspec_then `s.refs ++ junk ++ refs' ++ refs''` STRIP_ASSUME_TAC)
-\\ rw[]
-\\ FULL_SIMP_TAC pure_ss [GSYM APPEND_ASSOC]
-\\ `s.refs ++ (junk ++ (refs' ++ (refs'' ++ refs'''))) = s.refs ++ (junk ++ (refs' ++ refs'')) ++ refs'''` by simp[]
-\\ pop_assum(fn x => FULL_SIMP_TAC pure_ss [x])
-\\ first_x_assum(fn x => MATCH_MP evaluate_empty_state_IMP_junk x |> ASSUME_TAC)
-\\ fs[]
-\\ evaluate_unique_result_tac
-\\ rw[Once evaluate_cases]
-\\ evaluate_unique_result_tac
-\\ rw[Once evaluate_cases]
-\\ rw[do_app_def, store_alloc_def]
-\\ rw[namespaceTheory.nsOptBind_def]
-\\ rw[with_same_ffi]
-\\ qpat_abbrev_tac `loc = LENGTH junk + L`
-\\ last_x_assum(qspecl_then [`Loc loc`, `s with refs := s.refs ++ junk ++ refs' ++ refs'' ++ refs''' ++ [Refv u]`, `p`] ASSUME_TAC)
-\\ first_assum(fn x => let val a = concl x |> dest_imp |> fst in sg `^a` end)
->-(
-    rw[REFS_PRED_def]
-    \\ rw[GSYM STAR_ASSOC]
-    \\ rw[Once STAR_def]
-    \\ qexists_tac `store2heap_aux (LENGTH (s.refs ++ junk ++ refs' ++ refs'' ++ refs''')) [Refv u]`
-    \\ qexists_tac `st2heap p (s with refs := s.refs ++ junk ++ refs' ++ refs'' ++ refs''')`
-    \\ PURE_REWRITE_TAC[Once SPLIT_SYM]
-    \\ rw[STATE_SPLIT_REFS]
-    >-(
-	rw[REF_REL_def]
-	\\ rw[SEP_CLAUSES, SEP_EXISTS_THM]
-	\\ qexists_tac `u`
-        \\ EXTRACT_PURE_FACTS_TAC
-	\\ rw[REF_HPROP_SAT_EQ, cfStoreTheory.store2heap_aux_def])
-    \\ rw[Once (GSYM GC_STAR_GC), STAR_ASSOC]
-    \\ rw[Once STAR_def]
-    \\ qexists_tac `st2heap p (s with refs := s.refs)`
-    \\ qexists_tac `store2heap_aux (LENGTH s.refs) (junk ++ refs' ++ refs'' ++ refs''')`
-    \\ PURE_REWRITE_TAC[GSYM APPEND_ASSOC]
-    \\ rw[STATE_SPLIT_REFS, SAT_GC]
-    \\ fs[REFS_PRED_def, with_same_refs])
-\\ qpat_x_assum `A ==> R` IMP_RES_TAC
-\\ first_x_assum(qspec_then `[]` STRIP_ASSUME_TAC)
-\\ fs[merge_env_def]
-\\ Cases_on `env0`
-\\ Cases_on `n`
-\\ Cases_on `n0`
-\\ fs[namespaceTheory.nsBind_def, namespaceTheory.nsAppend_def]
-\\ evaluate_unique_result_tac
-\\ qexists_tac `refs2`
-\\ fs[REFS_PRED_FRAME_def]
-\\ rw[]
-\\ first_x_assum(qspec_then `F' * GC` ASSUME_TAC)
-\\ first_assum(fn x => let val a = concl x |> dest_imp |> fst in sg `^a` end)
->-(
-    rw[GSYM STAR_ASSOC]
-    \\ rw[Once STAR_def]
-    \\ qexists_tac `store2heap_aux (LENGTH (s.refs ++ junk ++ refs' ++ refs'' ++ refs''')) [Refv u]`
-    \\ qexists_tac `st2heap p (s with refs := s.refs ++ junk ++ refs' ++ refs'' ++ refs''')`
-    \\ PURE_REWRITE_TAC[Once SPLIT_SYM]
-    \\ rw[STATE_SPLIT_REFS]
-    >-(
-	rw[REF_REL_def]
-	\\ rw[SEP_CLAUSES, SEP_EXISTS_THM]
-	\\ qexists_tac `u`
-        \\ EXTRACT_PURE_FACTS_TAC
-	\\ rw[REF_HPROP_SAT_EQ, cfStoreTheory.store2heap_aux_def])
-    \\ rw[STAR_ASSOC]
-    \\ rw[Once STAR_def]
-    \\ qexists_tac `st2heap p (s with refs := s.refs)`
-    \\ qexists_tac `store2heap_aux (LENGTH s.refs) (junk ++ refs' ++ refs'' ++ refs''')`
-    \\ PURE_REWRITE_TAC[GSYM APPEND_ASSOC]
-    \\ rw[STATE_SPLIT_REFS, SAT_GC]
-    \\ fs[REFS_PRED_def, with_same_refs])
-\\ qpat_x_assum `A ==> R` IMP_RES_TAC
-\\ fs[GSYM STAR_ASSOC, GC_STAR_GC]
-\\ first_x_assum(fn x => PURE_ONCE_REWRITE_RULE[STAR_COMM] x |> ASSUME_TAC)
-\\ fs[STAR_ASSOC]
-\\ first_x_assum(fn x => MATCH_MP GC_ABSORB_R x |> ASSUME_TAC)
-\\ fs[]);
-
-val Eval_lookup_var = Q.store_thm("Eval_lookup_var",
-`!env vname xv x TYPE. nsLookup env.v (Short vname) = SOME xv ==>
-(Eval env (Var (Short vname)) (TYPE x) <=> TYPE x xv)`,
-rw[Eval_def]
-\\ EQ_TAC
->-(simp[Once evaluate_cases] \\ rw[] \\ metis_tac[])
-\\ rw[Once evaluate_cases]
-\\ rw[state_component_equality]);
-
-val STATE_REFS_TYPE_def = theorem"STATE_REFS_TYPE_def";
-
-val test_10_def = Define `test10 n m z refs = insert_monad (test9 n m z) refs`;
 
 val Long_tm = ``namespace$Long : tvarN -> (tvarN, tvarN) id -> (tvarN, tvarN) id ``;
 fun get_exn_constructs () = let
@@ -389,16 +227,112 @@ fun create_local_defs th = let
     in th' end
 
     val th = List.foldl create_fun_let th lookup_info
+
+    (* Instantiate the last environment variable *)
+    val empty_env = ``<| v := Bind [] []; c := Bind [] [] |> : v sem_env``
+    val th = Thm.INST [last_env |-> empty_env] th |> PURE_REWRITE_RULE [merge_env_bind_empty]
 in th end;
 
-fun translate_insert_monad def = let
+fun gen_name_tac name (g as (asl, w)) = let
+    val renamed_w_th = RENAME_VARS_CONV [name] w
+in (PURE_ONCE_REWRITE_TAC[renamed_w_th] \\ strip_tac) g end
+
+val H_STAR_emp = Q.prove(`H * emp = H`, simp[SEP_CLAUSES]);
+val emp_tm = ``set_sep$emp``;
+fun create_local_references th = let
+    val th = PURE_REWRITE_RULE[!H_def] th
+			      |> PURE_ONCE_REWRITE_RULE[GSYM H_STAR_emp]
+			      |> PURE_REWRITE_RULE[GSYM STAR_ASSOC]
+    (* Rename the state variable in the heap invariant *)
+    val state_var = concl th |> rator |> rand
+    val H_eq = ALPHA_CONV state_var (concl th |> rand)
+    val th = PURE_ONCE_REWRITE_RULE[H_eq] th
+
+    val P = concl th |> rator |> rator |> rand
+    val STATE_RI = get_type_inv (type_of state_var)
+
+    fun create_local_ref th = let
+	(* Instantiate the EvalSt theorem *)
+	val exp = concl th |> rator |> rator |> rator |> rand
+	val originalH = concl th |> rand
+	val H_part = dest_abs originalH |> snd
+	val (H_part1, H_part2) = dest_star H_part
+	val H_part2 = mk_abs(state_var, H_part2)
+
+	val state_field = rand H_part1
+	val get_ref_fun = mk_abs(state_var, state_field)
+	val Eval_state_field = hol2deep state_field
+	val field_expr = concl Eval_state_field |> rator |> rand
+	val TYPE = concl Eval_state_field |> rand |> rator
+
+	val refs_env = concl th |> rator |> rator |> rator |> rator |> rand
+	val loc_name = rator refs_env |> rator |> rand
+	val loc = rator refs_env |> rand
+	val env = rand refs_env
+
+	val gen_th = GEN loc th
+	val EvalSt_th = ISPECL[exp, field_expr, get_ref_fun, TYPE, loc_name, env, H_part2, P, state_var] EvalSt_Opref |> BETA_RULE
+
+	(* Retrieve the first assumption *)
+	val assum1 = concl EvalSt_th |> dest_imp |> fst
+	val assum1_env = assum1 |> rator |> rator |> rand
+
+	(* Prove the assumption about the state field expression *)
+	val Eval_state_field_env = concl Eval_state_field |> rator |> rator |> rand
+	val Eval_state_field = DISCH_ALL Eval_state_field
+					 |> Thm.INST[Eval_state_field_env |-> assum1_env]
+	val assum2 = concl Eval_state_field |> dest_imp |> fst
+	val lv_env = assum2 |> rator |> rator |> rand
+	val lv_vname = assum2 |> rator |> rand |> rand |> rand
+	val lv_x = assum2 |> rand |> rand
+	val lookup_th = EVAL ``nsLookup ^lv_env.v (Short ^lv_vname)``
+	val lv_xv = concl lookup_th |> rhs |> rand
+	val Eval_lookup_th = ISPECL [lv_env, lv_vname, lv_xv, lv_x, STATE_RI] Eval_lookup_var
+	val Eval_lookup_th = MP Eval_lookup_th lookup_th |> EQ_IMP_RULE |> snd |> UNDISCH
+	val Eval_state_field = MP Eval_state_field Eval_lookup_th
+	val assum3_th = concl Eval_state_field |> dest_imp |> fst |> EVAL |> EQT_ELIM
+	val Eval_state_field = MP Eval_state_field assum3_th
+
+	(* Simplify the first assumption *)
+	val EvalSt_th = MP EvalSt_th Eval_state_field
+
+	(* Simplify the second assumption *)
+	val EvalSt_th = MP EvalSt_th gen_th
+    in EvalSt_th end
+
+    fun create_local_refs_rec th = let
+	val originalH = concl th |> rand |> dest_abs |> snd
+    in if same_const originalH emp_tm then th
+       else create_local_refs_rec (create_local_ref th) end
+
+    val th = create_local_refs_rec th |> PURE_REWRITE_RULE[merge_env_bind_empty]
+
+    (* Transform the EvalSt predicate to an Eval predicate *)
+    val th = MATCH_MP EvalSt_to_Eval th
+in th end;
+
+fun apply_Eval_Fun (x, th) = let
+    val tms = FVL [x] empty_varset
+    val [assum] = List.filter (can (fn y => Term.raw_match [] tms ``A ^x xv`` y ([], []))) (hyp th)
+    val th = DISCH assum th
+    val v = rand assum
+    val th = GENL[v, x] th
+    val th = MATCH_MP Eval_Fun th
+in th end
+
+fun translate_run def = let
     (* Decompose the definition *)
-    val (def_lhs, def_rhs) = concl test_10_def |> strip_forall |> snd |> dest_eq
+    val (def_lhs, def_rhs) = concl def |> strip_forall |> snd |> dest_eq
+
+    val fname = repeat rator def_lhs |> dest_const |> fst |> get_unique_name
+    val _ = print ("Translating monadic " ^ fname ^ "for run\n")
+    val fname_str = stringLib.fromMLstring fname
+
     val Mvar = mk_var("M", ``:('a, 'b, 'c) M``)
     val Svar = mk_var("S", ``:'a``)
-    val (tms, tys) = match_term ``insert_monad ^Mvar ^Svar`` def_rhs
+    val (tms, tys) = match_term ``run ^Mvar ^Svar`` def_rhs
     val monad_tm = Term.subst tms (Term.inst tys Mvar)
-    val state_tm = Term.subst tms (Term.inst tys Svar)
+    val state_var = Term.subst tms (Term.inst tys Svar)
     val (monad_f, monad_params) = strip_comb monad_tm
 
     (* Construct the Eval predicates for the parameters *)
@@ -421,8 +355,18 @@ fun translate_insert_monad def = let
     val monad_th = List.foldl (fn (x, th) => MATCH_MP(MATCH_MP EvalM_ArrowM th) x)
 			      monad_th params_evals
 
-    (* Translate the insert_monad construct *)
+    (* Add the state parameter assumption *)
     val env = concl monad_th |> rator |> rator |> rator |> rand
+    val STATE_RI = get_type_inv (type_of state_var)
+    val state_var_name = stringLib.fromMLstring(dest_var state_var |> fst)
+    val Eval_state_var_assum = ``Eval ^env (Var (Short ^state_var_name)) (^STATE_RI ^state_var)``
+    val monad_th = ADD_ASSUM Eval_state_var_assum monad_th
+
+    (* Symplify the VALID_REFS_PRED assumption *)
+    val VALID_REFS_PRED_assum = ``VALID_REFS_PRED ^(!H)``
+    val monad_th = PURE_REWRITE_RULE[VALID_REFS_PRED_EvalM_simp] (DISCH VALID_REFS_PRED_assum monad_th)
+
+    (* Translate the run construct *)
     val x = concl monad_th |> rator |> rand |> rand
     val exp = concl monad_th |> rator |> rator |> rand
     val MONAD_TYPE = concl monad_th |> rator |> rand |> rator
@@ -434,20 +378,34 @@ fun translate_insert_monad def = let
     val th = case exn_module_name of
 		 SOME module_name =>
 		 ISPECL [cons_names, module_name, vname, TYPE, EXN_TYPE, x, exp,
-			 !H, state_tm, env] EvalM_insert_monad_MODULE
+			 !H, state_var, env] EvalM_run_MODULE
 	       | NONE =>
 		 ISPECL [cons_names, vname, TYPE, EXN_TYPE, x, exp,
-			 !H, state_tm, env] EvalM_insert_monad_SIMPLE
+			 !H, state_var, env] EvalM_run_SIMPLE
     (* Prove the assumptions *)
     val [EXN_assum, distinct_assum, vname_assum1, vname_assum2] = List.take(
 	    concl th |> strip_imp |> fst, 4)
     val EXN_th = prove(EXN_assum, rw[] \\ Cases_on `e` \\ fs[!EXN_TYPE_def_ref])
     val th = MP th EXN_th
 		
-    val distinct_rw = SIMP_CONV list_ss [] distinct_assum
-    val vname_rw1 = SIMP_CONV list_ss [] vname_assum1
-    val vname_rw2 = SIMP_CONV list_ss [] vname_assum2
-    val th = SIMP_RULE bool_ss [EXN_rw, distinct_rw, vname_rw1, vname_rw2] th
+    val distinct_th = SIMP_CONV list_ss [] distinct_assum |> EQT_ELIM
+    val vname_th1 = SIMP_CONV list_ss [] vname_assum1 |> EQT_ELIM
+    val vname_th2 = SIMP_CONV list_ss [] vname_assum2 |> EQT_ELIM
+
+    val EXC_TYPE_tm = get_type_inv ``:('a, 'b) exc`` |> rator |> rator
+    val EXC_TYPE_def = DB.find "EXC_TYPE_def" |> List.hd |> snd |> fst
+		       handle Empty => raise (ERR "m_translate_run" "The `exc` type needs to be registered in the current program")
+    val EXC_RI_prove_tac =
+	irule EQ_EXT \\ gen_name_tac "A"
+        \\ irule EQ_EXT \\ gen_name_tac "B"
+        \\ irule EQ_EXT \\ gen_name_tac "x"
+        \\ irule EQ_EXT \\ gen_name_tac "v"
+        \\ Cases_on `x`
+        \\ simp[EXC_TYPE_def, EXC_TYPE_aux_def]
+    val EXN_rw = prove(``EXC_TYPE_aux = ^EXC_TYPE_tm``, EXC_RI_prove_tac)
+
+    val th = List.foldl (fn (a, th) => MP th a) th [distinct_th, vname_th1, vname_th2]
+    val th = PURE_REWRITE_RULE[EXN_rw] th
     val th = MP th monad_th
 
     (* Undischarge the lookup assumptions *)
@@ -462,27 +420,28 @@ fun translate_insert_monad def = let
     (* Create the local function definitions *)
     val th = create_local_defs th
 
-    (* Remove the last environment *)
-    val empty_env = ``<| v := Bind [] []; c := Bind [] [] |> : v sem_env``
-    val th = Thm.INST [last_env |-> empty_env] th |> PURE_REWRITE_RULE [merge_env_bind_empty]
-
     (*
      * Instantiate the environment 0
      *)
     val global_env = get_env(get_curr_prog_state())
     val params_bindings = List.map(fn x => (concl x |> rator |> rator |> rand |> rand |> rand,
 					    concl x |> rator |> rand |> rand)) params_evals
-    val state_var = concl th |> rator |> rand
+    (* val state_var = concl th |> rator |> rand *)
     val state_var_eval = hol2deep state_var
-    val state_var_binding = ((concl state_var_eval |> rator |> rand |> rand |> rand), state_var)
+    val state_var_v = mk_var((dest_var state_var |> fst) ^"_v", ``:v``)
+    val state_var_vname = concl state_var_eval |> rator |> rand |> rand |> rand
+    val state_var_binding = (state_var_vname, state_var)
+    val state_var_binding_v = (state_var_vname, state_var_v)
+
+    val params_bindings = state_var_binding::(List.rev params_bindings)
     
     (* Create variables for the deep embeddings of the parameters *)
     val fvl = HOLset.listItems(FVL ((concl th)::(hyp th)) empty_varset)
-    val deep_params = List.map (fn (n, var) => variant fvl (mk_var((dest_var var |> fst) ^ "_v", ``:v``))) params_bindings
-    val hol_deep_pairs = List.map (fn ((n, x), xv) => (x, xv)) (zip params_bindings deep_params)
+    val params_v = List.map (fn (n, var) => variant fvl (mk_var((dest_var var |> fst) ^ "_v", ``:v``))) params_bindings
+    val hol_deep_pairs = List.map (fn ((n, x), xv) => (x, xv)) (zip params_bindings params_v)
     val deep_params_map = List.foldr (fn ((x, xv), m) => Redblackmap.insert(m, x, xv)) (Redblackmap.mkDict Term.compare) hol_deep_pairs
 
-    val params_bindings_v = List.map (fn ((n, x), xv) => (n, xv)) (zip params_bindings deep_params)
+    val params_bindings_v = List.map (fn ((n, x), xv) => (n, xv)) (zip params_bindings params_v)
     val params_bindings_v = List.map mk_pair params_bindings_v
     val params_bindings_v = mk_list(params_bindings_v, ``:tvarN # v``)
 
@@ -499,8 +458,17 @@ fun translate_insert_monad def = let
     val th = List.foldr (fn (a, th) => MP (DISCH (concl a) th) a) th lookup_cons_rws
     val assums = hyp th
     val nsLookup_assums = List.filter (can (match_term ``nsLookup env id = SOME var``)) assums
-    val nsLookup_assums_rws = mapfilter(fn x => EVAL x |> EQT_ELIM) nsLookup_assums
+    fun Eval_error_msg x = let
+	val vname = lhs x |> rand |> rand
+	val msg1 = "Error with the binding: "
+	val msg2 = stringLib.fromHOLstring vname
+	val msg3 = " - check that the proper functions and types are defined in the current CakeML program"
+    in msg1 ^msg2 ^msg3 end
+    val nsLookup_assums_rws = mapfilter(fn x => EVAL x |> EQT_ELIM handle HOL_ERR _ => raise (ERR "m_translate_run" (Eval_error_msg x))) nsLookup_assums
+
     val th = List.foldr (fn (a, th) => MP (DISCH (concl a) th) a) th nsLookup_assums_rws
+    
+    (* Symplify the assumption parameters *)
     val assums = hyp th
     val Eval_var_assums = List.filter (can (match_term ``Eval env exp (P x)``)) assums
 
@@ -514,102 +482,40 @@ fun translate_insert_monad def = let
 	val rw_th = ISPECL[env, vname, xv, x, TYPE] Eval_lookup_var
 	val rw_th_assum = concl rw_th |> dest_imp |> fst
 	val rw_th = MP rw_th (EVAL rw_th_assum |> EQT_ELIM)
-
+		       
 	val inv_to_eval = EQ_IMP_RULE rw_th |> snd |> UNDISCH
 	val th = MP (DISCH (concl inv_to_eval) th) inv_to_eval
     in th end
 
     val th = List.foldl rewrite_Eval_var th Eval_var_assums
-
-			(* Create the store *)
-
-
-
-Eval_def
-
-DB.apropos ``(x <=> T) <=> x``
-
-EVAL ``lookup_cons "Success" (merge_env auto_env_9 init_env)``
-``lookup_cons``
-
-val assum1 = List.nth(assums, 1)
-EVAL assum1
-
-    val assums = DISCH_ALL th' 
-    val clean_assumptions (DISCH_ALL th')
-
-lookup_cons_def
-
-EVAL ``NUM x y``
-    val all_param_bindings = List.map mk_pair all_param_bindings
-    val all_params_bindings = mk_list(all_param_bindings, ``:tvarN # v``)
-    val env0 = ``merge_env
-
-    val th' = Thm.INST[local_environment_var_0  |-> global_env] th |> DISCH_ALL
-
+			|> PURE_REWRITE_RULE[Bind_list_to_write]
 
     (* Create the store *)
-    fun create_local_store th = let
-	val th = PURE_REWRITE_RULE [!H_def, GSYM STAR_ASSOC] th
-	val state_var = concl th |> rator |> rand
+    val th = create_local_references th
 
-th
-EvalSt_Opref
+    (* Abstract the parameters *)
+    val th = PURE_REWRITE_RULE [GSYM def] th
+    val rev_params = List.map snd params_bindings
+    val th = List.foldl apply_Eval_Fun th rev_params
 
-assums
-List.hd assums
+    (* Expand the handle_mult expression *)
+    val th = PURE_REWRITE_RULE[handle_mult_def, handle_one_def] th
 
-fun create_local_store refs_init_list arrays_init_list store_hprop_name =
-  let
-      val _ = if List.null refs_init_list andalso List.null arrays_init_list
-	      then raise (ERR "create_store" "need a non empty list of reference init values")
-	      else ()
+    (* Store the spec *)
+    val th = PURE_REWRITE_RULE[Eval_Fun_rw] th
+    val fname = repeat rator def_lhs |> dest_const |> fst |> get_unique_name
+    val v = th |> concl |> rand |> rator |> rand
+    val e = th |> concl |> rand |> rand
+    val v_name = find_const_name (fname ^ "_v")
+    val _ = ml_prog_update (add_Dlet_Fun fname_str v e v_name)
+    val s = get_curr_prog_state ()
+    val v_def = hd (get_v_defs s)
+    val th = th |> REWRITE_RULE [GSYM v_def]
 
-      val initial_state = mk_var("s", ``:unit semanticPrimitives$state``)
-      val initial_store = ``^initial_state.refs``
-      val initial_env = get_env(get_ml_prog_state())
-
-      (* Allocate the references *)
-      fun create_ref ((name, def), (s, env)) =
-	let
-	    val trans_th = abs_translate def
-	    val expr = rator (concl trans_th) |> rand
-	    val e = ``(App Opref [^expr])``
-	    (derive_eval_thm name e)
-
-
-	    val value_expr = 
-	    val init_name = concl def |> dest_eq |> fst |> dest_const |> fst
-	    val init_name = stringLib.fromMLstring init_name
-	    val e = ``(App Opref [Var (Short ^init_name)])``
-	    val _ = ml_prog_update (add_Dlet (derive_eval_thm name e) name [])
-	    val ref_def = DB.fetch (current_theory()) (name ^ "_def")
-	in
-	    (value_def, ref_def)
-	end
-      val ref_name_def_pairs = List.map (fn (n, d, _, _) => (n, d)) refs_init_list
-      val refs_trans_results = List.map create_ref ref_name_def_pairs
-
-      (* Allocate the arrays *)
-      fun create_array (name, def) =
-	let
-	    val init_name = concl def |> lhs |> dest_const |> fst
-
-	    val (array_v_def, array_loc_def, ref_def, eval_th) =
-		derive_eval_thm_ALLOCATE_EMPTY_ARRAY init_name def
-	    val _ = ml_prog_update(add_Dlet eval_th name [])
-         in
-	     (array_v_def, array_loc_def, ref_def)
-	end
-      val array_name_def_pairs = List.map (fn (n, d, _, _, _, _, _, _) => (n, d)) arrays_init_list
-      val arrays_trans_results = List.map create_array array_name_def_pairs
-  in
-    (initial_store, refs_trans_results, arrays_trans_results)
-  end;
-
-hol2deep ``state_refs x_3 x_2 x_1:state_refs``
-
-
-Net.listItems (!dynamic_specs)
+    (* Store the certificate for later use *)
+    val pre = TRUTH
+    val _ = add_v_thms (fname,fname,th,pre)
+    val th = save_thm(fname ^ "_v_thm",th)
+in th end
 
 val _ = export_theory ();
